move code from swap.v into reusable files

bedrock2/src/bedrock2Examples/LiveVerif/swap.v
@@ -5,6 +5,8 @@ Require Import coqutil.Datatypes.PropSet.
 Require Import coqutil.Datatypes.Inhabited.
 Require Import coqutil.Tactics.letexists coqutil.Tactics.Tactics coqutil.Tactics.rewr coqutil.Tactics.rdelta.
 Require Import Coq.Program.Tactics.
+Require Import coqutil.Tactics.ltac_list_ops.
+Require Import coqutil.Tactics.autoforward.
 Require Import coqutil.Map.Interface coqutil.Map.Properties coqutil.Map.OfListWord.
 Require coqutil.Map.SortedListString. (* for function env, other maps are kept abstract *)
 Require Import coqutil.Word.Interface coqutil.Word.Properties.
@@ -20,13 +22,8 @@ Require Import coqutil.Word.Bitwidth32.
 Require Import Coq.Strings.String.
 Require Import bedrock2Examples.LiveVerif.string_to_ident.
 Require Import bedrock2Examples.LiveVerif.ident_to_string.
-Import List.ListNotations. Local Open Scope list_scope.
-
-Ltac destruct_bools :=
-  repeat match goal with
-         | H: context[if ?b then _ else _] |- _ =>
-             let t := type of b in constr_eq t bool; destruct b
-         end.
+Require Import bedrock2.SepBulletPoints.
+Require Import bedrock2.SepAutoArray bedrock2.SepAuto.
 
 (* `vpattern x in H` is like `pattern x in H`, but x must be a variable and is
    used as the binder in the lambda being created *)
@@ -50,203 +47,6 @@ Fixpoint ands(Ps: list Prop): Prop :=
 Lemma ands_nil: ands nil. Proof. cbn. auto. Qed.
 Lemma ands_cons: forall [P: Prop] [Ps: list Prop], P -> ands Ps -> ands (P :: Ps).
 Proof. cbn. auto. Qed.
-
-
-Require Import Coq.Program.Tactics.
-Require Import coqutil.Tactics.autoforward.
-
-Ltac fwd_rewrites ::= fwd_rewrite_db_in_star.
-
-#[export] Hint Rewrite
-  List.firstn_all2
-  List.skipn_all2
-  List.firstn_eq_O
-  List.skipn_eq_O
-  Nat.min_l
-  Nat.min_r
-using ZnWords : fwd_rewrites.
-
-Inductive get_option{A: Type}: option A -> (A -> Prop) -> Prop :=
-| mk_get_option: forall (a: A) (post: A -> Prop), post a -> get_option (Some a) post.
-
-Module Import SepLogPredsWithAddrLast. Section __.
-  Context {width : Z} {word : Word.Interface.word width} {mem : map.map word byte}.
-
-  Definition at_addr(addr: word)(clause: word -> mem -> Prop): mem -> Prop := clause addr.
-
-  (* Redefinitions to change order of arguments to put address last *)
-
-  Definition ptsto_bytes (n : nat) (value : tuple byte n) (addr : word) : mem -> Prop :=
-    ptsto_bytes n addr value.
-
-  Definition littleendian (n : nat) (value : Z) (addr : word) : mem -> Prop :=
-    littleendian n addr value.
-
-  Definition truncated_scalar sz (value : Z) addr : mem -> Prop :=
-    truncated_scalar sz addr value.
-
-  Definition truncated_word sz (value: word) addr : mem -> Prop :=
-    truncated_word sz addr value.
-
-  Definition scalar16 := truncated_word Syntax.access_size.two.
-  Definition scalar32 := truncated_word Syntax.access_size.four.
-  Definition scalar := truncated_word Syntax.access_size.word.
-
-  Definition word_array(vs: list word)(addr: word): mem -> Prop :=
-    array Scalars.scalar (word.of_Z (bytes_per_word width)) addr vs.
-End __. End SepLogPredsWithAddrLast.
-
-(* `*` is at level 40, and we want to bind stronger than `*`,
-   and moreover, `^` is at level 30, and for consistency, we also want to bind stronger than `^`,
-   so we choose 25 *)
-Notation "addr |-> clause" := (at_addr addr clause)
-  (at level 25,
-   format "addr  |->  '[' clause ']'").
-
-Section SepLog.
-  Context {word: word.word 32} {mem: map.map word byte}.
-  Context {word_ok: word.ok word} {mem_ok: map.ok mem}.
-
-  Lemma load_of_sep_cps: forall sz addr value R m (post: word -> Prop),
-      sep (addr |-> truncated_word sz value) R m /\ post (truncate_word sz value) ->
-      get_option (Memory.load sz m addr) post.
-  Proof.
-    intros. destruct H. eapply load_of_sep in H. rewrite H.
-    constructor. assumption.
-  Qed.
-
-  Lemma load_word_of_sep_cps: forall addr value R m (post: word -> Prop),
-      sep (addr |-> scalar value) R m /\ post value ->
-      get_option (Memory.load Syntax.access_size.word m addr) post.
-  Proof.
-    intros. destruct H. eapply load_word_of_sep in H. rewrite H.
-    constructor. assumption.
-  Qed.
-
-  Lemma store_word_of_sep_cps_two_subgoals: forall addr oldvalue newvalue R m (post: mem -> Prop),
-      seps [addr |-> scalar oldvalue; R] m ->
-      (forall m', seps [addr |-> scalar newvalue; R] m' -> post m') ->
-      get_option (Memory.store access_size.word m addr newvalue) post.
-  Proof.
-    intros. eapply Scalars.store_word_of_sep in H. 2: eassumption.
-    destruct H as (m1 & E & P). rewrite E. constructor. exact P.
-  Qed.
-
-  Lemma store_word_of_sep_cps: forall addr oldvalue newvalue R m (post: mem -> Prop),
-      seps [addr |-> scalar oldvalue; R;
-            emp (forall m', seps [addr |-> scalar newvalue; R] m' -> post m')] m ->
-      get_option (Memory.store access_size.word m addr newvalue) post.
-  Proof.
-    intros. unfold seps in H. apply sep_assoc in H. apply sep_emp_r in H. destruct H.
-    eapply store_word_of_sep_cps_two_subgoals. 1: unfold seps. 1: eassumption. eassumption.
-  Qed.
-
-  (* R, typically instantiated to `seps [whatever; is; left]`, appears twice:
-     On the left of the impl1 (this determines its value), and as the first
-     element of the `seps` on the right (there, it is an evar for the frame).
-     P is the continuation postcondition. *)
-  Lemma impl1_done: forall (R: mem -> Prop) (P: Prop),
-      P -> impl1 R (seps [R; emp P]).
-  Proof.
-    unfold impl1, seps. intros. apply sep_emp_r. auto.
-  Qed.
-
-  (* All arguments except stmt are just ghost parameters to guide typeclass search.
-     The shape of stmt will typically be
-       forall valAll valPart valFrame1 ... valFrameN,
-         sidecondition saying that assembling valPart valFrame1 ... valFrameN = valAll ->
-         iff1 (seps [addrPart |-> predPart valPart; Frame...]) (addrAll |-> predAll valAll)
-     but since that's a variable number of universally quantified variables, it would
-     be a bit cumbersome to enforce that shape, and since it's not needed to enforce it,
-     we don't. *)
-  Definition split_sepclause{TypeAll TypePart: Type}
-             (addrAll : word)(predAll : TypeAll  -> word -> mem -> Prop)
-             (addrPart: word)(predPart: TypePart -> word -> mem -> Prop)
-             (stmt: Prop) := stmt.
-
-  Lemma access_scalar_in_word_array: forall a a',
-      word.unsigned (word.sub a' a) mod 4 = 0 ->
-      split_sepclause a word_array a' scalar
-        (let i := Z.to_nat (word.unsigned (word.sub a' a) / 4) in
-         forall vs vs1 v vs2,
-           (* connected with /\ because it needs to be solved by considering both at once *)
-           vs = vs1 ++ [v] ++ vs2 /\ List.length vs1 = i ->
-           iff1 (seps [a |-> word_array vs1;
-                       a' |-> scalar v;
-                       word.add a (word.of_Z (4 * Z.of_nat (S i))) |-> word_array vs2])
-                (a |-> word_array vs)).
-  Proof.
-    unfold split_sepclause.
-    unfold word_array, scalar, truncated_word, Scalars.scalar, at_addr, seps.
-    intros. destruct H0. subst vs.
-    cbn [List.app].
-    symmetry.
-    etransitivity.
-    1: eapply array_append.
-    cbn [array].
-    change (bytes_per_word _) with 4.
-    cancel.
-    cancel_seps_at_indices 0%nat 0%nat. {
-      f_equal. ZnWords.
-    }
-    cancel_seps_at_indices 0%nat 0%nat. {
-      f_equal. ZnWords.
-    }
-    reflexivity.
-  Qed.
-
-  Local Set Warnings "-notation-overridden".
-  Local Infix "++" := SeparationLogic.app. Local Infix "++" := app : list_scope.
-  Let nth n xs := SeparationLogic.hd (emp(map:=mem) True) (SeparationLogic.skipn n xs).
-  Let remove_nth n (xs : list (mem -> Prop)) :=
-    (SeparationLogic.firstn n xs ++ SeparationLogic.tl (SeparationLogic.skipn n xs)).
-
-  Lemma rewrite_ith_in_lhs_of_impl1: forall i Ps Pi Qs R,
-      nth i Ps = Pi ->
-      iff1 (seps Qs) Pi -> (* <-- used right-to-left *)
-      impl1 (seps (remove_nth i Ps ++ Qs)) R ->
-      impl1 (seps Ps) R.
-  Proof.
-    intros. subst Pi.
-    unfold nth, remove_nth in *.
-    rewrite <-(seps_nth_to_head i Ps).
-    rewrite <- H0.
-    rewrite 2seps_app in H1. rewrite seps_app.
-    etransitivity. 2: eassumption.
-    ecancel.
-  Qed.
-End SepLog.
-
-Create HintDb split_sepclause_goal.
-
-#[export] Hint Extern 1 (split_sepclause _ word_array _ scalar _) =>
-  eapply access_scalar_in_word_array; destruct_bools; ZnWords : split_sepclause_goal.
-
-Section WithA.
-  Context {A: Type}.
-
-  Lemma list_expose_nth{inhA: inhabited A}: forall (vs: list A) i,
-      (i < List.length vs)%nat ->
-      vs = List.firstn i vs ++ [List.nth i vs default] ++ List.skipn (S i) vs /\
-        List.length (List.firstn i vs) = i.
-  Proof.
-    intros. rewrite List.firstn_nth_skipn by assumption.
-    rewrite List.firstn_length_le by Lia.lia. auto.
-  Qed.
-End WithA.
-
-Create HintDb split_sepclause_sidecond.
-
-#[export] Hint Extern 1 (_ = ?l ++ [_] ++ _ /\ List.length ?l = _) =>
-  eapply list_expose_nth; destruct_bools; ZnWords : split_sepclause_sidecond.
-
-Create HintDb merge_sepclause_sidecond.
-
-#[export] Hint Extern 1 (@eq (list _) ?listL ?listR /\ @eq nat ?lenL ?lenR) =>
-  assert_fails (has_evar lenL);
-  assert_fails (has_evar lenR);
-  is_evar listL; split; [reflexivity|destruct_bools; ZnWords]
-: merge_sepclause_sidecond.
 
 Section WithParams.
   Import bedrock2.Syntax.
@@ -779,170 +579,6 @@ Notation "[ x ; y ; .. ; z ]" :=
 Notation "l" := (arguments_marker l)
   (at level 100, only printing) : live_scope.
 
-Module Import MySepNotations.
-
-Declare Scope sep_list_scope.
-Delimit Scope sep_list_scope with sep_list.
-
-Notation "* x * y * .. * z" :=
-  (@cons (@map.rep _ _ _ -> Prop) x
-    (@cons (@map.rep _ _ _ -> Prop) y
-      .. (@cons (@map.rep _ _ _ -> Prop) z nil) .. ))
-  (at level 39, x at level 39, y at level 39, z at level 39,
-   (* starting with a space to make sure we never create an opening comment *)
-   format " '[v' *  x  '//' *  y  '//' *  ..  '//' *  z  ']'")
-  : sep_list_scope.
-
-Notation "* x" :=
-  (@cons (@map.rep _ _ _ -> Prop) x nil)
-  (at level 39, x at level 39,
-   (* starting with a space to make sure we never create an opening comment *)
-   format " '[v' *  x ']'")
-  : sep_list_scope.
-
-Notation "m 'satisfies' <{ l }>" := (seps l%sep_list m)
-  (at level 10,
-   format "'[v' m  'satisfies'  <{ '//'  l '//' }> ']'")
-  : live_scope.
-
-Notation "<{ l1 }> ==> <{ l2 }>" := (impl1 (seps l1%sep_list) (seps l2%sep_list))
-  (at level 10,
-   format "'[v' <{ l1 '//' }>  ==>  <{ '//'   l2 '//' }> ']'")
-  : live_scope.
-
-Notation "<{ l1 }> <==> <{ l2 }>" := (iff1 (seps l1%sep_list) (seps l2%sep_list))
-  (at level 10,
-   format "'[v' <{ l1 '//' }>  <==>  <{ '//'   l2 '//' }> ']'")
-  : live_scope.
-
-End MySepNotations.
-
-Section NotationTests.
-  Context {width : Z} {word : Word.Interface.word width} {mem : map.map word byte}.
-
-  Goal Some (fun (a b: word) (v: word) =>
-               seps ( * (a |-> scalar v) * (b |-> scalar v) * (emp True) )%sep_list) = None.
-  Abort.
-
-  Goal (forall (a b: word) (v: word) (current_mem: mem),
-          seps ( * a |-> scalar v * b |-> scalar v * emp True )%sep_list current_mem).
-  Proof. intros. (*
-  Note how `satisfies` does not increase the indentation of the `*` bullet points,
-  each bullet point is indented by just two spaces:
-
-  current_mem satisfies <{
-    * a |-> scalar v
-    * b |-> scalar v
-    * emp True
-  }>
-  *)
-  match goal with |- ?G => enough G as M end. Abort.
-
-  Context (a b c d e f g h: word) (frobnicate: word -> word -> word) (v: word).
-
-  Let manyseps := (
-     * a |-> scalar v * b |-> scalar v * emp True * c |-> scalar v
-     * d |->  scalar v
-     * e |-> scalar (frobnicate (frobnicate (frobnicate v (frobnicate v v)) (frobnicate
-          (frobnicate v (frobnicate v v)) (frobnicate v (frobnicate v v)))) (frobnicate v v))
-     * f |-> scalar v
-     * (frobnicate (frobnicate (frobnicate v (frobnicate v v)) (frobnicate
-          (frobnicate v (frobnicate v v)) (frobnicate v (frobnicate v v)))) (frobnicate v v)) |->
-       scalar v
-     * h |-> (scalar v) * emp True
-     * (frobnicate (frobnicate (frobnicate v (frobnicate v v)) (frobnicate
-          (frobnicate v (frobnicate v v)) (frobnicate v (frobnicate v v)))) (frobnicate v v)) |->
-       scalar (frobnicate (frobnicate (frobnicate v (frobnicate v v)) (frobnicate
-          (frobnicate v (frobnicate v v)) (frobnicate v (frobnicate v v)))) (frobnicate v v))
-  )%sep_list.
-
-  Goal forall (a b c d e f g h: word) (frobnicate: word -> word -> word) (v: word) (m: mem),
-     m satisfies <{ manyseps }>.
-  Proof.
-    intros. subst manyseps. match goal with |- ?G => enough G end.
-  Abort.
-
-  Goal forall (a b: word) (v: word),
-    <{ * a |-> scalar v
-       * b |-> scalar v
-       * emp True
-    }> ==> <{
-       * b |-> scalar v
-       * a |-> scalar v
-    }>.
-  Proof. intros. match goal with |- ?G => enough G end. Abort.
-
-  Goal forall (a b: word) (v: word),
-    <{ manyseps }> ==> <{
-       * b |-> scalar v
-       * a |-> scalar v
-    }>.
-  Proof. intros. subst manyseps. match goal with |- ?G => enough G end. Abort.
-
-  Goal forall (a b: word) (v: word),
-    <{ manyseps }> <==> <{
-       * b |-> scalar v
-       * a |-> scalar v
-    }>.
-  Proof. intros. subst manyseps. match goal with |- ?G => enough G end. Abort.
-
-End NotationTests.
-
-Ltac clear_split_sepclause_stack :=
-  repeat match goal with
-         | H: split_sepclause _ _ _ _ _ |- _ => clear H
-         end.
-
-Ltac pop_split_sepclause_stack :=
-  let H := lazymatch goal with H: seps _ ?m |- wp_cmd _ _ _ ?m _ _ => H end in
-  let Sp := lazymatch goal with Sp: split_sepclause _ _ _ _ _ |- _ => Sp end in
-  ((cbv [split_sepclause] in Sp;
-    cbn [seps] in Sp, H;
-    seprewrite_in_by Sp H ltac:(eauto with merge_sepclause_sidecond)
-   ) || let T := type of Sp in idtac "Note: Failed to merge sep clauses using" T);
-  clear Sp.
-
-Ltac impl_ecancel_step_with_splitting :=
-  lazymatch goal with
-  | |- Lift1Prop.impl1 (seps ?L) (seps ((?addrR |-> ?predR ?valR) :: ?RRest)) =>
-    let iLi := index_and_element_of L in (* <-- multi-success! *)
-    let i := lazymatch iLi with (?i, _) => i end in
-    let Li := lazymatch iLi with (_, ?Li) => Li end in
-    let Li := eval cbn [hd app firstn tl skipn] in Li in
-    lazymatch Li with
-    (* Simplifying assumption: Only the last argument to predL is a value that
-       can be changed by stores and function calls, all other arguments are constants *)
-    | ?addrL |-> ?predL ?valL =>
-        let Sp := fresh "Sp" in
-        eassert (split_sepclause addrL predL addrR predR _) as Sp
-            (* typeclasses eauto instead of eauto because eauto unfolds split_sepclause
-               and then just does `exact H` for the last Prop in the context, and it
-               seems that `Hint Opaque` and `Hint Constants Opaque` don't fix that
-               (and `Opaque split_sepclause` would fix it, but also affects the conversion
-               algorithm) *)
-            by typeclasses eauto with split_sepclause_goal;
-        eapply (rewrite_ith_in_lhs_of_impl1 i L Li);
-        cbn [hd app firstn tl skipn];
-        [ reflexivity
-        | cbv [split_sepclause] in Sp;
-          eapply Sp;
-          solve [eauto with split_sepclause_sidecond]
-        | ]
-    end
-  end.
-
-Ltac ecancel_with_remaining_emp_Prop :=
-  cancel_seps;
-  repeat (repeat ecancel_step_by_implication; try impl_ecancel_step_with_splitting);
-  refine (impl1_done _ _ _).
-
-Ltac ecancel_assumption_with_remaining_emp_Prop :=
-  match goal with
-  | H: seps _ ?m |- seps _ ?m =>
-    refine (Morphisms.subrelation_refl Lift1Prop.impl1 _ _ _ m H)
-  end;
-  ecancel_with_remaining_emp_Prop.
-
 Ltac simpli_step :=
   match goal with
   | H: ?x = ?y |- _ => is_var x; is_var y; subst x
@@ -961,11 +597,6 @@ Ltac simpli_step_in_goal :=
     rewrite word.unsigned_of_Z_nowrap by Lia.lia
   | _ => progress groundcbv_in_goal
   end.
-
-Ltac is_fresh x := assert_succeeds (pose proof tt as x).
-
-Ltac make_fresh x :=
-  tryif is_fresh x then idtac else let x' := fresh x "_0" in rename x into x'.
 
 Ltac put_into_current_locals is_decl :=
   lazymatch goal with
@@ -1000,14 +631,6 @@ Ltac put_into_current_locals is_decl :=
     end
   end.
 
-Ltac map_with_ltac f l :=
-  lazymatch l with
-  | ?h :: ?t =>
-    let t' := map_with_ltac f t in
-    let h' := f h in constr:(h' :: t')
-  | nil => open_constr:(@nil _)
-  end.
-
 Ltac eval_expr_step :=
   lazymatch goal with
   | |- wp_expr _ _ (expr.load access_size.word _) _ => eapply wp_load_word
@@ -1022,6 +645,8 @@ Ltac eval_expr_step :=
   | |- wp_expr _ _ (expr.op _ _ _) _ => eapply wp_op; cbv [interp_binop]
   end.
 
+Ltac eval_expr := repeat eval_expr_step.
+
 Ltac eval_dexpr_step :=
   lazymatch goal with
   | |- dexpr_bool_prop _ _ (expr.lazy_and _ _) _ =>
@@ -1033,6 +658,8 @@ Ltac eval_dexpr_step :=
   | |- dexpr _ _ (expr.var _) _ => eapply dexpr_var; reflexivity
   | |- dexpr _ _ (expr.literal _) _ => eapply dexpr_literal
   end.
+
+Ltac eval_dexpr := repeat eval_dexpr_step.
 
 Ltac start :=
   lazymatch goal with
@@ -1591,17 +1218,6 @@ Ltac pull_dlet_and_exists_step :=
       destruct H as [x H]
   end.
 
-Ltac find_in_list test Ps :=
-  lazymatch Ps with
-  | ?h :: ?t =>
-      lazymatch test h with
-      | true => constr:((0%nat, h))
-      | false => lazymatch find_in_list test t with
-                 | (?i, ?P) => constr:((S i, P))
-                 end
-      end
-  end.
-
 Ltac merge_pair H Ps Qs is_match lem := once (
   lazymatch index_and_element_of Ps with
   | (?i, ?P) =>
@@ -1628,12 +1244,6 @@ Ltac same_lhs P Q :=
       end
   end.
 
-Ltac constr_eqb x y :=
-  lazymatch x with
-  | y => constr:(true)
-  | _ => constr:(false)
-  end.
-
 Ltac same_addr_and_pred P Q :=
   lazymatch P with
   | ?a |-> ?pred _ =>
@@ -1656,6 +1266,12 @@ Ltac seps_about_same_mem x y :=
                  | seps _ ?m => constr:(true)
                  | _ => constr:(false)
                  end
+  | _ => constr:(false)
+  end.
+
+Ltac constr_eqb x y :=
+  lazymatch x with
+  | y => constr:(true)
   | _ => constr:(false)
   end.
 
@@ -1706,7 +1322,7 @@ Inductive snippet :=
 
 Ltac assign is_decl name val :=
   eapply (wp_set _ name val);
-  repeat eval_expr_step;
+  eval_expr;
   [.. (* maybe some unsolved side conditions *)
   | try ((* to simplify value that will become bound with :=, at which point
             rewrites will not apply any more *)
@@ -1714,20 +1330,19 @@ Ltac assign is_decl name val :=
          repeat simpli_step_in_goal;
          put_into_current_locals is_decl) ].
 
-(* TODO change order of definitions so that this hook is not needed any more *)
-Ltac flatten_seps := fail "not yet implemented".
-Ltac transfer_sep_order := fail "not yet implemented".
-
 Ltac store sz addr val :=
   eapply (wp_store _ addr val);
-  repeat eval_expr_step;
+  eval_expr;
   [.. (* maybe some unsolved side conditions *)
   | lazymatch goal with
     | |- forall (_: @map.rep _ _ _), seps _ _ -> _ =>
         intros;
         repeat pop_split_sepclause_stack;
-        flatten_seps;
-        transfer_sep_order
+        lazymatch goal with
+        | HOld: seps _ ?mOld, HNew: _ ?mNew |- wp_cmd _ _ _ ?mNew _ _ =>
+            flatten_seps_in HNew;
+            transfer_sep_order_from_to HOld HNew
+        end
     | |- _ => idtac (* expression evaluation did not work fully automatically *)
     end ].
 
@@ -1735,7 +1350,7 @@ Ltac cond c :=
   lazymatch goal with
   | |- wp_cmd _ _ ?t ?m (reconstruct ?vars ?vals) _ =>
     eapply (wp_if_bool_dexpr _ c vars vals);
-    [ repeat eval_dexpr_step
+    [ eval_dexpr
     | let b := fresh "Scope0" in pose proof (mk_scope_marker ThenBranch) as b; intro
     | let b := fresh "Scope0" in pose proof (mk_scope_marker ElseBranch) as b; intro
     | ]
@@ -1763,7 +1378,7 @@ Ltac prove_final_post :=
     repeat match goal with
            | x := _ |- _ => subst x
            end;
-    destruct_bools;
+    destruct_bool_vars;
     repeat match goal with
            | H: ands (_ :: _) |- _ => destruct H
            | H: ands [] |- _ => clear H
@@ -1966,32 +1581,6 @@ Tactic Notation "#" constr(s) := add_snippet s; after_snippet.
 
 Set Ltac Backtrace.
 
-Require Import Coq.Sorting.Permutation Coq.Sorting.Sorting.
-
-Module FstNatOrder <: Orders.TotalLeBool.
-  Definition t: Type := nat * nat.
-  Definition leb: t -> t -> bool :=
-    fun '(x, _) '(y, _) => Nat.leb x y.
-  Theorem leb_total: forall a1 a2, leb a1 a2 = true \/ leb a2 a1 = true.
-  Proof.
-    unfold leb. intros [x _] [y _]. destr (x <=? y)%nat. 1: auto.
-    right. apply Nat.leb_le. unfold lt in E. eapply Nat.le_trans. 2: exact E.
-    do 2 constructor.
-  Qed.
-End FstNatOrder.
-
-Module FstNatSorting := Sort FstNatOrder.
-
-Lemma iff1_refl{A: Type}(P: A -> Prop): iff1 P P. Proof. reflexivity. Qed.
-Lemma iff1_sym{A: Type}{P Q: A -> Prop}: iff1 P Q -> iff1 Q P.
-Proof. intros. symmetry. assumption. Qed.
-
-Ltac iff1_syntactic_reflexivity :=
-  lazymatch goal with
-  | |- iff1 ?x ?y => first [is_evar x | is_evar y | constr_eq x y]
-  end;
-  exact (iff1_refl _).
-
 (* COQBUG (performance) https://github.com/coq/coq/issues/10743#issuecomment-530673037
    Probably fixed on master *)
 Ltac cond_hyp_factor :=
@@ -2012,9 +1601,11 @@ Ltac adhoc_lia_performance_fixes :=
   cond_hyp_factor;
   subst.
 
+Require Import Coq.Sorting.Permutation.
+
 Load LiveVerif.
 Import SepLogPredsWithAddrLast.
-Import MySepNotations.
+Import bedrock2.SepBulletPoints.
 (* to re-override Notations loaded trough `Load LiveVerif/bedrock2.Map.SeparationLogic` *)
 
 (* Note: If you re-import ZnWords after this, you'll get the old better_lia again *)
@@ -2024,234 +1615,6 @@ Ltac better_lia ::=
   Lia.lia.
 
 Local Set Default Goal Selector "1".
-
-Lemma seps'_Permutation: forall (l1 l2: list (mem -> Prop)),
-    Permutation l1 l2 -> iff1 (seps' l1) (seps' l2).
-Proof.
-  induction 1.
-  - reflexivity.
-  - simpl. rewrite IHPermutation. reflexivity.
-  - simpl. cancel.
-  - etransitivity; eassumption.
-Qed.
-
-Lemma seps_Permutation: forall (l1 l2: list (mem -> Prop)),
-    Permutation l1 l2 -> iff1 (seps l1) (seps l2).
-Proof.
-  intros.
-  etransitivity. 2: eapply seps'_iff1_seps.
-  etransitivity. 2: eapply seps'_Permutation; exact H.
-  symmetry. eapply seps'_iff1_seps.
-Qed.
-
-Fixpoint zip_with_counter{A: Type}(l: list A)(start: nat): list (A * nat) :=
-  match l with
-  | nil => nil
-  | x :: xs => (x, start) :: zip_with_counter xs (S start)
-  end.
-
-Definition zip_with_index{A: Type}(l: list A): list (A * nat) := zip_with_counter l 0.
-
-Lemma snd_zip_with_counter: forall {A: Type} (l: list A) (start: nat),
-    List.map snd (zip_with_counter l start) = List.seq start (List.length l).
-Proof. induction l; simpl; intros. 1: reflexivity. f_equal. apply IHl. Qed.
-
-Lemma snd_zip_with_index: forall {A: Type} (l: list A),
-    List.map snd (zip_with_index l) = List.seq 0 (List.length l).
-Proof. intros. apply snd_zip_with_counter. Qed.
-
-Lemma List__map_nth_seq_self{A: Type}(d: A)(l: list A):
-  List.map (fun i => List.nth i l d) (List.seq 0 (List.length l)) = l.
-Proof.
-  induction l; cbn -[List.nth]. 1: reflexivity.
-  unfold List.nth at 1.
-  f_equal.
-  etransitivity. 2: exact IHl.
-  rewrite <- List.seq_shift.
-  rewrite List.map_map.
-  reflexivity.
-Qed.
-
-(* redefinitions so that cbv on it does not cbv user-defined terms *)
-Definition my_list_map{A B: Type}(f: A -> B): list A -> list B :=
-  Eval unfold List.map in (List.map f).
-Definition my_list_nth{A: Type}: nat -> list A -> A -> A :=
-  Eval unfold List.nth in (@List.nth A).
-
-Definition apply_permutation_with_default(p: list nat){A: Type}(l: list A)(d: A): list A :=
-  my_list_map (fun i => my_list_nth i l d) p.
-
-Definition apply_permutation(p: list nat){A: Type}(l: list A): list A :=
-  match l with
-  | nil => nil
-  | cons d _ => apply_permutation_with_default p l d
-  end.
-
-Lemma apply_permutation_with_default_is_Permutation: forall (p: list nat) A (l: list A) d,
-    Permutation p (List.seq 0 (List.length l)) ->
-    Permutation l (apply_permutation_with_default p l d).
-Proof.
-  unfold apply_permutation_with_default. intros.
-  eapply Permutation_trans. 2: {
-    eapply Permutation_map.
-    eapply Permutation_sym.
-    exact H.
-  }
-  rewrite List__map_nth_seq_self.
-  apply Permutation_refl.
-Qed.
-
-Lemma apply_permutation_is_Permutation: forall (p: list nat) (A: Type) (l: list A),
-    Permutation p (List.seq 0 (List.length l)) ->
-    Permutation l (apply_permutation p l).
-Proof.
-  intros. unfold apply_permutation. destruct l.
-  - apply Permutation_refl.
-  - apply apply_permutation_with_default_is_Permutation. assumption.
-Qed.
-
-Definition order_to_permutation(order: list nat): list nat :=
-  List.map snd (FstNatSorting.sort (zip_with_index order)).
-
-Lemma order_to_permutation_is_Permutation(order: list nat):
-    Permutation (order_to_permutation order) (List.seq 0 (List.length order)).
-Proof.
-  unfold order_to_permutation.
-  eapply Permutation_trans. {
-    eapply Permutation_map.
-    eapply Permutation_sym.
-    eapply FstNatSorting.Permuted_sort.
-  }
-  rewrite snd_zip_with_index.
-  eapply Permutation_refl.
-Qed.
-
-(* `order` and `l` must have the same length.
-    The i-th element of `order` is the sort key of the i-th element of `l`.
-    Returns `l` sorted according to these sort keys. *)
-Definition reorder(order: list nat){A: Type}(l: list A): list A :=
-  apply_permutation (order_to_permutation order) l.
-
-Lemma reorder_is_iff1: forall (order: list nat) (l: list (mem -> Prop)),
-    List.length order = List.length l ->
-    iff1 (seps l) (seps (reorder order l)).
-Proof.
-  intros.
-  apply seps_Permutation.
-  unfold reorder.
-  apply apply_permutation_is_Permutation.
-  rewrite <- H.
-  apply order_to_permutation_is_Permutation.
-Qed.
-
-(* for lists with concrete structure/length, but elements that should not be cbv'd *)
-Ltac list_length l :=
-  lazymatch l with
-  | nil => constr:(O)
-  | cons _ ?tail => let r := list_length tail in constr:(S r)
-  end.
-
-Ltac clause_index clause clauses start_index default_index :=
-  lazymatch clauses with
-  | cons (at_addr ?a _) ?tail =>
-    lazymatch clause with
-    | at_addr a _ => constr:(start_index)
-    | _ => clause_index clause tail (S start_index) default_index
-    end
-  | cons clause _ => constr:(start_index)
-  | cons _ ?tail => clause_index clause tail (S start_index) default_index
-  | nil => constr:(default_index)
-  end.
-
-Ltac get_order_rec old_clauses new_clauses default_index :=
-  lazymatch new_clauses with
-  | nil => constr:(@nil nat)
-  | cons ?clause ?tail =>
-    let priority := clause_index clause old_clauses 0%nat default_index in
-    let rest := get_order_rec old_clauses tail priority in
-    constr:(priority :: rest)
-  end.
-
-Ltac get_order old_clauses new_clauses :=
-  (* if the first clause is not found in old_clauses, we put it at the end;
-     if a non-first clause is not found, we put it after the clause that's
-     to the left of it in new_clauses, so we give it the same priority value,
-     so the returned order might have duplicate priority values, and we rely
-     on mergesort being stable to keep the order between clauses of the same priority *)
-  let n := list_length old_clauses in
-  get_order_rec old_clauses new_clauses n.
-
-Ltac flatten_seps ::=
-  lazymatch goal with
-  | HNew: ?new_nested ?mNew |- wp_cmd _ _ _ ?mNew _ _ =>
-    let tmem := type of mNew in
-    let E := fresh "E" in
-    eassert (@iff1 tmem new_nested _) as E;
-    [ (* from `new_nested` to `Tree.to_sep tree` *)
-      let stars := eval cbn[seps] in new_nested in
-      let tree := reify stars in
-      transitivity (Tree.to_sep tree); [
-        cbn [seps Tree.to_sep Tree.interp]; iff1_syntactic_reflexivity
-      |];
-      (* from `Tree.to_sep tree` to `seps (Tree.flatten tree)` *)
-      transitivity (seps (Tree.flatten tree)); [
-        exact (iff1_sym (Tree.flatten_iff1_to_sep tree))
-      |];
-      (* from `seps (Tree.flatten tree)` to `seps new_clauses` *)
-      cbn [SeparationLogic.Tree.flatten SeparationLogic.Tree.interp SeparationLogic.app];
-      iff1_syntactic_reflexivity
-    | let HNewNew := fresh in pose proof (proj1 (E mNew) HNew) as HNewNew;
-      clear E HNew;
-      rename HNewNew into HNew ]
-  end.
-
-(* Given an old and a new sep hyp, transfers the order of the sepclauses from the old one
-   to the new one *)
-Ltac transfer_sep_order ::=
-  lazymatch goal with
-  | HOld: seps ?old_clauses ?mOld, HNew: seps ?new_clauses ?mNew |- wp_cmd _ _ _ ?mNew _ _ =>
-    let tmem := type of mNew in
-    let E := fresh "E" in
-    eassert (@iff1 tmem (seps new_clauses) _) as E;
-    [ (* from `seps new_clauses` to `seps (reorder order new_clauses)` *)
-      let order := get_order old_clauses new_clauses in
-      etransitivity; [
-        eapply (reorder_is_iff1 order new_clauses); reflexivity
-      |];
-      (* from `seps (reorder order new_clauses)` to cbv'd version of it *)
-      cbv [reorder];
-      let r := eval vm_compute in (order_to_permutation order) in
-          change (order_to_permutation order) with r;
-      cbv [apply_permutation apply_permutation_with_default my_list_map my_list_nth];
-      reflexivity
-    | let HNewNew := fresh in pose proof (proj1 (E mNew) HNew) as HNewNew;
-      clear E HOld HNew;
-      try clear mOld;
-      make_fresh mOld;
-      rename HNewNew into HOld, mNew into mOld ]
-  end.
-
-Lemma reordering_test: forall addr1 addr2 addr3 addr4 v1_old v1_new v2 v3 v4 R (m m': mem)
-                              fs t l c post,
-    seps [addr1 |-> scalar v1_old; addr2 |-> scalar v2; addr3 |-> scalar v3; R] m ->
-    (* value at addr1 was updated, addr2 was consumed, addr4 was added, and order was changed: *)
-    seps [R; seps [addr3 |-> scalar v3; addr4 |-> scalar v4]; addr1 |-> scalar v1_new] m' ->
-    (* desired order:
-    seps [addr1 |-> scalar v1_new; addr3 |-> scalar v3; addr4 |-> scalar v4; R] m1 *)
-    True ->
-    wp_cmd (call fs) c t m' l post.
-Proof.
-  intros *. intros M M2 ExtraHyp.
-          (* 0                        1                    2                    3
-  M  : seps [addr1 |-> scalar v1_old; addr2 |-> scalar v2; addr3 |-> scalar v3; R] m0
-  M2 : seps [R; addr3 |-> scalar v3; addr4 |-> scalar v4; addr1 |-> scalar v1_new] m1
-  order :=  [3; 2;                   2;                   0                      ] *)
-  flatten_seps.
-  transfer_sep_order.
-  lazymatch type of M with
-  | seps [addr1 |-> scalar v1_new; addr3 |-> scalar v3; addr4 |-> scalar v4; R] m => idtac
-  end.
-Abort.
 
 Tactic Notation ".*" constr(s) "*" := add_snippet s; after_snippet.
 
