bedrock2/src/bedrock2/SepAutoArray.v
@@ -1,0 +1,89 @@
+Require Import bedrock2.SepAuto.
+Require Import bedrock2.Array.
+
+Section SepLog32. (* TODO try to generalize to any width without breaking automation *)
+  Context {word: word.word 32} {mem: map.map word byte}.
+  Context {word_ok: word.ok word} {mem_ok: map.ok mem}.
+
+  Definition word_array(vs: list word)(addr: word): mem -> Prop :=
+    array Scalars.scalar (word.of_Z 4) addr vs.
+
+  Lemma access_scalar_in_word_array: forall a a',
+      word.unsigned (word.sub a' a) mod 4 = 0 ->
+      split_sepclause a word_array a' scalar
+        (let i := Z.to_nat (word.unsigned (word.sub a' a) / 4) in
+         forall vs vs1 v vs2,
+           (* connected with /\ because it needs to be solved by considering both at once *)
+           vs = vs1 ++ [v] ++ vs2 /\ List.length vs1 = i ->
+           iff1 (seps [a |-> word_array vs1;
+                       a' |-> scalar v;
+                       word.add a (word.of_Z (4 * Z.of_nat (S i))) |-> word_array vs2])
+                (a |-> word_array vs)).
+  Proof.
+    unfold split_sepclause.
+    unfold word_array, scalar, truncated_word, Scalars.scalar, at_addr, seps.
+    intros. destruct H0. subst vs.
+    cbn [List.app].
+    symmetry.
+    etransitivity.
+    1: eapply array_append.
+    cbn [array].
+    cancel.
+    cancel_seps_at_indices 0%nat 0%nat. {
+      f_equal. ZnWords.
+    }
+    cancel_seps_at_indices 0%nat 0%nat. {
+      f_equal. ZnWords.
+    }
+    reflexivity.
+  Qed.
+End SepLog32.
+
+Section WithA.
+  Context {A: Type}.
+
+  Lemma list_expose_nth{inhA: inhabited A}: forall (vs: list A) i,
+      (i < List.length vs)%nat ->
+      vs = List.firstn i vs ++ [List.nth i vs default] ++ List.skipn (S i) vs /\
+        List.length (List.firstn i vs) = i.
+  Proof.
+    intros. rewrite List.firstn_nth_skipn by assumption.
+    rewrite List.firstn_length_le by Lia.lia. auto.
+  Qed.
+End WithA.
+
+Ltac destruct_bool_vars :=
+  repeat match goal with
+         | H: context[if ?b then _ else _] |- _ =>
+             is_var b; let t := type of b in constr_eq t bool; destruct b
+         end.
+
+(* Three hints in three different DBs indicating how to find the rewrite lemma,
+   how to solve its sideconditions for the split direction, and how to solve its
+   sideconditions for the merge direction: *)
+
+#[export] Hint Extern 1 (split_sepclause _ word_array _ scalar _) =>
+  eapply access_scalar_in_word_array; destruct_bool_vars; ZnWords
+: split_sepclause_goal.
+
+#[export] Hint Extern 1 (_ = ?l ++ [_] ++ _ /\ List.length ?l = _) =>
+  eapply list_expose_nth; destruct_bool_vars; ZnWords
+: split_sepclause_sidecond.
+
+#[export] Hint Extern 1 (@eq (list _) ?listL ?listR /\ @eq nat ?lenL ?lenR) =>
+  assert_fails (has_evar lenL);
+  assert_fails (has_evar lenR);
+  is_evar listL; split; [reflexivity|destruct_bool_vars; ZnWords]
+: merge_sepclause_sidecond.
+
+
+(* Hints to simplify/cleanup the expressions that were created by repeated
+   splitting and merging of sep clauses: *)
+#[export] Hint Rewrite
+  List.firstn_all2
+  List.skipn_all2
+  List.firstn_eq_O
+  List.skipn_eq_O
+  Nat.min_l
+  Nat.min_r
+using ZnWords : fwd_rewrites.
