bedrock2/src/bedrock2/SepBulletPoints.v
@@ -1,0 +1,122 @@
+(* Notations to display a list of separation logic predicates as a bullet point list *)
+
+Require Import coqutil.Map.Interface coqutil.Word.Interface.
+Require Import bedrock2.Lift1Prop.
+Require Import bedrock2.Map.Separation.
+
+Declare Scope sep_list_scope.
+Delimit Scope sep_list_scope with sep_list.
+
+Notation "* x * y * .. * z" :=
+  (@cons (@map.rep _ _ _ -> Prop) x
+    (@cons (@map.rep _ _ _ -> Prop) y
+      .. (@cons (@map.rep _ _ _ -> Prop) z nil) .. ))
+  (at level 39, x at level 39, y at level 39, z at level 39,
+   (* starting with a space to make sure we never create an opening comment *)
+   format " '[v' *  x  '//' *  y  '//' *  ..  '//' *  z  ']'")
+  : sep_list_scope.
+
+Notation "* x" :=
+  (@cons (@map.rep _ _ _ -> Prop) x nil)
+  (at level 39, x at level 39,
+   (* starting with a space to make sure we never create an opening comment *)
+   format " '[v' *  x ']'")
+  : sep_list_scope.
+
+Declare Scope seps_impl_scope.
+Open Scope seps_impl_scope.
+
+Notation "m 'satisfies' <{ l }>" := (seps l%sep_list m)
+  (at level 10,
+   format "'[v' m  'satisfies'  <{ '//'  l '//' }> ']'")
+  : seps_impl_scope.
+
+Notation "<{ l1 }> ==> <{ l2 }>" := (impl1 (seps l1%sep_list) (seps l2%sep_list))
+  (at level 10,
+   format "'[v' <{ l1 '//' }>  ==>  <{ '//'   l2 '//' }> ']'")
+  : seps_impl_scope.
+
+Notation "<{ l1 }> <==> <{ l2 }>" := (iff1 (seps l1%sep_list) (seps l2%sep_list))
+  (at level 10,
+   format "'[v' <{ l1 '//' }>  <==>  <{ '//'   l2 '//' }> ']'")
+  : seps_impl_scope.
+
+
+Section NotationTests.
+  Context {width : BinInt.Z} {word : Word.Interface.word width}
+          {mem : map.map word Byte.byte}.
+
+  (* local, just for testing, real definition is elsewhere *)
+  Let at_addr(addr: word)(clause: word -> mem -> Prop): mem -> Prop := clause addr.
+  Local Notation "addr |-> clause" := (at_addr addr clause)
+    (at level 25, format "addr  |->  '[' clause ']'").
+
+  Context (scalar: word -> word -> mem -> Prop).
+
+  Goal Some (fun (a b: word) (v: word) =>
+               seps ( * (a |-> scalar v) * (b |-> scalar v) * (emp True) )%sep_list) = None.
+  Abort.
+
+  Goal (forall (a b: word) (v: word) (current_mem: mem),
+          seps ( * a |-> scalar v * b |-> scalar v * emp True )%sep_list current_mem).
+  Proof. intros. (*
+  Note how `satisfies` does not increase the indentation of the `*` bullet points,
+  each bullet point is indented by just two spaces:
+
+  current_mem satisfies <{
+    * a |-> scalar v
+    * b |-> scalar v
+    * emp True
+  }>
+  *)
+  match goal with |- ?G => enough G as M end. Abort.
+
+  Context (a b c d e f g h: word) (frobnicate: word -> word -> word) (v: word).
+
+  Let manyseps := (
+     * a |-> scalar v * b |-> scalar v * emp True * c |-> scalar v
+     * d |->  scalar v
+     * e |-> scalar (frobnicate (frobnicate (frobnicate v (frobnicate v v)) (frobnicate
+          (frobnicate v (frobnicate v v)) (frobnicate v (frobnicate v v)))) (frobnicate v v))
+     * f |-> scalar v
+     * (frobnicate (frobnicate (frobnicate v (frobnicate v v)) (frobnicate
+          (frobnicate v (frobnicate v v)) (frobnicate v (frobnicate v v)))) (frobnicate v v)) |->
+       scalar v
+     * h |-> (scalar v) * emp True
+     * (frobnicate (frobnicate (frobnicate v (frobnicate v v)) (frobnicate
+          (frobnicate v (frobnicate v v)) (frobnicate v (frobnicate v v)))) (frobnicate v v)) |->
+       scalar (frobnicate (frobnicate (frobnicate v (frobnicate v v)) (frobnicate
+          (frobnicate v (frobnicate v v)) (frobnicate v (frobnicate v v)))) (frobnicate v v))
+  )%sep_list.
+
+  Goal forall (a b c d e f g h: word) (frobnicate: word -> word -> word) (v: word) (m: mem),
+     m satisfies <{ manyseps }>.
+  Proof.
+    intros. subst manyseps. match goal with |- ?G => enough G end.
+  Abort.
+
+  Goal forall (a b: word) (v: word),
+    <{ * a |-> scalar v
+       * b |-> scalar v
+       * emp True
+    }> ==> <{
+       * b |-> scalar v
+       * a |-> scalar v
+    }>.
+  Proof. intros. match goal with |- ?G => enough G end. Abort.
+
+  Goal forall (a b: word) (v: word),
+    <{ manyseps }> ==> <{
+       * b |-> scalar v
+       * a |-> scalar v
+    }>.
+  Proof. intros. subst manyseps. match goal with |- ?G => enough G end. Abort.
+
+  Goal forall (a b: word) (v: word),
+    <{ manyseps }> <==> <{
+       * b |-> scalar v
+       * a |-> scalar v
+    }>.
+  Proof. intros. subst manyseps. match goal with |- ?G => enough G end. Abort.
+
+End NotationTests.
